<?xml version="1.0"?>
<pretext xmlns:xi="http://www.w3.org/2001/XInclude">
  <xi:include href="slidesinfo.ptx"/>
  <slideshow>
    <title>Induction</title>
    <subtitle>(Section 2.5)</subtitle>
    <section>
      <title>Recursive Reasoning</title>
      <slide>
        <title>Investigate!</title>       
          <p permid="Xka">
        What is the last digit of <m>6^n</m> in terms of <m>n</m>?
      </p>
      <p pause="yes">
        What if you knew the last digit of <m>6^{418}</m>.  Could you find the last digit of <m>6^{419}</m>?
      </p>
      <p pause="yes">
        How can we turn this recursive reasoning into a proof?
      </p>
      </slide>
    </section>
    <section>
      <title>Formalizing Proofs</title>
      <slide>
          <title>Induction Proof Structure</title>
          <p permid="bTT">
        Start by saying what the statement is that you want to prove: <q>Let <m>P(n)</m> be the statement<ellipsis/></q> To prove that <m>P(n)</m> is true for all <m>n \ge 0</m>, you must prove two facts:

        <ol permid="zcP"><li permid="DMI">
            <p permid="oDK">
              Base case: Prove that <m>P(0)</m> is true.
              You do this directly.
              This is often easy.
            </p>
          </li><li permid="jTR">
            <p permid="UKT">
              Inductive case: Prove that
              <m>P(k) \imp P(k+1)</m> for all <m>k \ge 0</m>.
              That is, prove that for any <m>k \ge 0</m> if <m>P(k)</m> is true,
              then <m>P(k+1)</m> is true as well.
              This is the proof of an if
              <ellipsis/> then
              <ellipsis/> statement,
              so you can assume <m>P(k)</m> is true (<m>P(k)</m> is called the
              <em>inductive hypothesis</em>).
                <idx><h>inductive hypothesis</h></idx>
            You must then explain why <m>P(k+1)</m> is also true, given that assumption.
            </p>
          </li></ol>
      </p>
          <p permid="Ibc">
        Assuming you are successful on both parts above,
        you can conclude,
        <q>Therefore by the principle of mathematical induction,
        the statement <m>P(n)</m> is true for all <m>n \ge 0</m>.</q>
      </p>
      </slide>
    </section>
    <section>
      <title>Examples</title>
      <slide>
        <example source-number="2.5.1">
          <statement>
            <p permid="SAh">
          Prove for each natural number <m>n \ge 1</m> that <m>1 + 2 + 3 + \cdots + n = \frac{n(n+1)}{2}</m>.
        </p>
          </statement>
        </example>
      </slide>
      <slide>
        <title>Proof</title>
        
        
          <p permid="tth">
            Let <m>P(n)</m> be the statement <m>1 + 2 + 3 + \cdots + n = \frac{n(n+1)}{2}</m>.
            We will show that <m>P(n)</m> is true for all natural numbers <m>n \ge 1</m>.
          </p>

          <p pause="yes">
            Base case: <m>P(1)</m> is the statement
            <m>1 = \frac{1(1+1)}{2}</m> which is clearly true.
          </p>
      </slide>
      <slide>
        <title>Proof Continued.</title>
        
        
          <p>
            Inductive case: Let <m>k \ge 1</m> be a natural number.
            Assume (for induction) that <m>P(k)</m> is true.
            That means <m>1 + 2 + 3 + \cdots + k = \frac{k(k+1)}{2}</m>.
            We will prove that <m>P(k+1)</m> is true as well.
            That is, we must prove that <m>1 + 2 + 3 + \cdots + k + (k+1) = \frac{(k+1)(k+2)}{2}</m>.
            To prove this equation,
            start by adding <m>k+1</m> to both sides of the inductive hypothesis:
            <me permid="htk">
              1 + 2 + 3 + \cdots + k + (k+1) = \frac{k(k+1)}{2} + (k+1)
            </me>.
          </p>

          <p pause="yes">
            Now, simplifying the right side we get:
            <md permid="NAt">
              <mrow>\frac{k(k+1)}{2} + k+1 \amp = \frac{k(k+1)}{2} + \frac{2(k+1)}{2}</mrow>
              <mrow>\amp = \frac{k(k+1) + 2(k+1)}{2}</mrow>
              <mrow>\amp = \frac{(k+2)(k+1)}{2}</mrow>
            </md>.
          </p>

          <p pause="yes">
            Thus <m>P(k+1)</m> is true,
            so by the principle of mathematical induction <m>P(n)</m> is true for all natural numbers <m>n \ge 1</m>.
          </p>
      </slide>
      <slide>
        <example source-number="2.5.2">
          <statement>
            <p permid="yHq">
          Prove that for all <m>n \in \N</m>,
          <m>6^n - 1</m> is a multiple of 5.
        </p>
          </statement>
        </example>
      </slide>
      <slide>
        <example source-number="2.5.3">
          <statement>
            <p permid="eOz">
          Prove that <m>n^2 \lt 2^n</m> for all integers <m>n \ge 5</m>.
        </p>
          </statement>
        </example>
      </slide>
    </section>
    <section>
      <title>Strong Induction</title>
      <slide>
        <title>Chocolate!</title>
        
        
          <p permid="Drj">
        How many times do you need to break a 4 by 6 chocolate bar to reduce it to single squares?
      </p>
      

            <p pause="yes">
          Conjecture: Given a <m>n</m>-square rectangular chocolate bar,
          it always takes <m>n-1</m> breaks to reduce the bar to single squares.
        </p>
        <p pause="yes">
          Idea: if you break an <m>n</m>-square bar into two smaller rectangles, of size <m>j</m> and <m>k</m>, then it takes <m>1 + (j-1) + (k-1)</m> total breaks.  But this is <m>n-1</m> breaks!
        </p>
      </slide>

      <slide>
          <title>Strong Induction Proof Structure</title>
          <p permid="oil">
        Again, start by saying what you want to prove:
        <q>Let <m>P(n)</m> be the statement<ellipsis/></q>
        Then establish two facts:

        <ol permid="fjY"><li permid="Qba">
            <p permid="ASc">
              Base case: Prove that <m>P(0)</m> is true.
            </p>
          </li><li permid="wij">
            <p permid="gZl">
              Inductive case: Assume <m>P(k)</m> is true for all <m>k \lt n</m>.
              Prove that <m>P(n)</m> is true.
            </p>
          </li></ol>

        Conclude, <q>therefore, by strong induction,
        <m>P(n)</m> is true for all <m>n \gt 0</m>.</q>
      </p>
      </slide>
      <slide>
        <example source-number="2.5.5">
          <statement>
            <p permid="KVI">
          Prove that any natural number greater than 1 is either prime
          or can be written as the product of primes.
        </p>
          </statement>
        </example>
      </slide>
    </section>
  </slideshow>
</pretext>
