<?xml version="1.0"?>
<pretext xmlns:xi="http://www.w3.org/2001/XInclude">
  <xi:include href="slidesinfo.ptx"/>
  <slideshow>
    <title>Solving Recurrence Relations</title>
    <subtitle>(Section 2.4)</subtitle>
    <introduction>
    <slide>
      
        <p permid="GOF">
        Consider the recurrence relation
        <me permid="elW">
          a_n = 5a_{n-1} - 6a_{n-2}
        </me>.
        <ol permid="tQt"><li permid="ZXC">
            <p permid="yAm">
              What sequence do you get if the initial conditions are <m>a_0 = 1</m>,
              <m>a_1 = 2</m>?
              Give a closed formula for this sequence.
            </p>
          </li><li permid="GeL">
            <p permid="eHv">
              What sequence do you get if the initial conditions are <m>a_0 = 1</m>,
              <m>a_1 = 3</m>?
              Give a closed formula.
            </p>
          </li><li permid="mlU">
            <p permid="KOE">
              What if <m>a_0 = 2</m> and <m>a_1 = 5</m>?
              Find a closed formula.
            </p>
          </li></ol>
      </p>
    </slide>
    
    <slide>
      <example source-number="2.4.1">
        <statement>
          <p permid="pQu">
          Find a recurrence relation and initial conditions for <m>1, 5, 17, 53, 161, 485\ldots</m>.
        </p>
        </statement>
      </example>
    </slide>
    <slide>
      <example source-number="2.4.2">
        <statement>
          <p permid="VXD">
          Check that <m>a_n = 2^n + 1</m> is a solution to the recurrence relation <m>a_n = 2a_{n-1} - 1</m> with <m>a_1 = 3</m>.
        </p>
        </statement>
      </example>
    </slide>
    </introduction>
    <section>
    <title>Telescoping and Iteration</title>
    
    
    <slide>
    <title>Telescoping</title>
    
    
    <p permid="TiB">
      <term>Telescoping</term>
      refers to the phenomenon when many terms in a large sum cancel out - so the sum
      <q>telescopes.</q> For example:
      <me permid="ykr">
        (2 - 1) + (3 - 2) + (4 - 3) + \cdots + (100 - 99) + (101 - 100) = -1 + 101
      </me>
      because every third term looks like:
      <m>2 + -2 = 0</m>, and then <m>3 + -3 = 0</m> and so on.
    </p>
    </slide>
    
    <slide>
      
      <example source-number="2.4.3">
        <statement>
          <p permid="CeM">
          Solve the recurrence relation
          <m>a_n = a_{n-1} + n</m> with initial term <m>a_0 = 4</m>.
        </p>
        </statement>
      </example>
    </slide>
    <slide>
    <title>Iteration</title>
    <p>
      What do you do when the left-hand side doesn't telescope?  <term>Iterate</term>: repeatedly find the next term and simplify.
    </p>
    
      <example source-number="2.4.4">
        <statement>
          <p permid="ilV">
          Use iteration to solve the recurrence relation <m>a_n = a_{n-1} + n</m> with <m>a_0 = 4</m>.
        </p>
        </statement>
      </example>
    </slide>
    <slide>
      <example source-number="2.4.5">
        <statement>
          <p permid="Ote">
          Solve the recurrence relation
          <m>a_n = 3a_{n-1} + 2</m> subject to <m>a_0 = 1</m>.
        </p>
        </statement>
      </example>
    </slide>
    </section>

    <section>
      <title>The Characteristic Root Technique</title>

      <slide>
        <p permid="QnV">
      Suppose we want to solve  <m>a_n = a_{n-1} + 6a_{n-2}</m>.
      
      Iteration is too complicated,
      but think just for a second what would happen if we <em>did</em> iterate.
      Perhaps the solution will take the form <m>r^n</m> for some constant <m>r</m>.
        </p>

        <p pause="yes">
      What happens if we plug in <m>r^n</m> into the recursion above?
      We get
          <me permid="TSv">
        r^n - r^{n-1} - 6r^{n-2} = 0
          </me>.
        </p>

        <p pause="yes">
      Now solve for <m>r</m>:
          <me permid="zZE">
        r^{n-2}(r^2 - r - 6) = 0
          </me>,
      so by factoring, <m>r = -2</m> or <m>r = 3</m>
     
      This tells us that <m>a_n = (-2)^n</m> is a solution to the recurrence relation,
      as is <m>a_n = 3^n</m>.
      </p>
      <p pause="yes">
        
      In fact, for any <m>a</m> and <m>b</m>,
          <m>a_n = a(-2)^n + b 3^n</m> is a solution.

      To find the values of <m>a</m> and <m>b</m>,
      use the initial conditions.
        </p>
      </slide>


      <slide>

          <title>Characteristic Roots</title>
          <p permid="cwJ">
        Given a recurrence relation <m>a_n + \alpha a_{n-1} + \beta a_{n-2} = 0</m>, the
        <term>characteristic polynomial</term> is
        <me permid="zUa">
          x^2 + \alpha x + \beta
        </me>
        giving the
        <term>characteristic equation</term>:
        <me permid="gbj">
          x^2 + \alpha x + \beta = 0
        </me>.
      </p>
          <p pause="yes">
        If <m>r_1</m> and <m>r_2</m> are two distinct roots of the characteristic polynomial (i.e, solutions to the characteristic equation),
        then the solution to the recurrence relation is
        <me permid="Mis">
          a_n = ar_1^n + br_2^n
        </me>,
        where <m>a</m> and <m>b</m> are constants determined by the initial conditions.
      </p>
      </slide>

      <slide>
        <example source-number="2.4.6">
          <statement>
            <p permid="uAn">
          Solve the recurrence relation
          <m>a_n = 7a_{n-1} - 10 a_{n-2}</m> with <m>a_0 = 2</m> and <m>a_1 = 3</m>.
        </p>
          </statement>
        </example>
      </slide>
      <slide>

          <title>Characteristic Root Technique for Repeated Roots</title>
          <p permid="oLb">
        Suppose the recurrence relation
        <m>a_n = \alpha a_{n-1} + \beta a_{n-2}</m> has a characteristic polynomial with only one root <m>r</m>.
        Then the solution to the recurrence relation is
        <me permid="QSl">
          a_n = ar^n + bnr^n
        </me>
        where <m>a</m> and <m>b</m> are constants determined by the initial conditions.
      </p>
        
      </slide>
      <slide>
        <example source-number="2.4.7">
          <statement>
            <p permid="aHw">
          Solve the recurrence relation
          <m>a_n = 6a_{n-1} - 9a_{n-2}</m> with initial conditions <m>a_0 = 1</m> and <m>a_1 = 4</m>.
        </p>
          </statement>
        </example>
      </slide>
    </section>
  </slideshow>
</pretext>
