<?xml version="1.0"?>
<pretext xmlns:xi="http://www.w3.org/2001/XInclude">
  <xi:include href="slidesinfo.ptx"/>
  <slideshow>
    <title>Solving Recurrence Relations</title>
    <slide>
      <investigation>
        <p permid="GOF">
        Consider the recurrence relation
        <me permid="elW">
          a_n = 5a_{n-1} - 6a_{n-2}
        </me>.
        <ol permid="tQt"><li permid="ZXC">
            <p permid="yAm">
              What sequence do you get if the initial conditions are <m>a_0 = 1</m>,
              <m>a_1 = 2</m>?
              Give a closed formula for this sequence.
            </p>
          </li><li permid="GeL">
            <p permid="eHv">
              What sequence do you get if the initial conditions are <m>a_0 = 1</m>,
              <m>a_1 = 3</m>?
              Give a closed formula.
            </p>
          </li><li permid="mlU">
            <p permid="KOE">
              What if <m>a_0 = 2</m> and <m>a_1 = 5</m>?
              Find a closed formula.
            </p>
          </li></ol>
      </p>
      </investigation>
    </slide>
    <slide>
      <example source-number="2.4.1">
        <statement>
          <p permid="pQu">
          Find a recurrence relation and initial conditions for <m>1, 5, 17, 53, 161, 485\ldots</m>.
        </p>
        </statement>
      </example>
    </slide>
    <slide>
      <example source-number="2.4.2">
        <statement>
          <p permid="VXD">
          Check that <m>a_n = 2^n + 1</m> is a solution to the recurrence relation <m>a_n = 2a_{n-1} - 1</m> with <m>a_1 = 3</m>.
        </p>
        </statement>
      </example>
    </slide>
    <slide>
      <example source-number="2.4.3">
        <statement>
          <p permid="CeM">
          Solve the recurrence relation
          <m>a_n = a_{n-1} + n</m> with initial term <m>a_0 = 4</m>.
        </p>
        </statement>
      </example>
    </slide>
    <slide>
      <example source-number="2.4.4">
        <statement>
          <p permid="ilV">
          Use iteration to solve the recurrence relation <m>a_n = a_{n-1} + n</m> with <m>a_0 = 4</m>.
        </p>
        </statement>
      </example>
    </slide>
    <slide>
      <example source-number="2.4.5">
        <statement>
          <p permid="Ote">
          Solve the recurrence relation
          <m>a_n = 3a_{n-1} + 2</m> subject to <m>a_0 = 1</m>.
        </p>
        </statement>
      </example>
    </slide>
    <subsection>
      <title>The Characteristic Root Technique</title>
      <slide>
        <assemblage>
          <title>Characteristic Roots</title>
          <p permid="cwJ">
            <idx><h>characteristic roots</h></idx>
        Given a recurrence relation <m>a_n + \alpha a_{n-1} + \beta a_{n-2} = 0</m>, the
        <term>characteristic polynomial</term> is
        <me permid="zUa">
          x^2 + \alpha x + \beta
        </me>
        giving the
        <term>characteristic equation</term>:
        <me permid="gbj">
          x^2 + \alpha x + \beta = 0
        </me>.
      </p>
          <p permid="IDS">
        If <m>r_1</m> and <m>r_2</m> are two distinct roots of the characteristic polynomial (i.e, solutions to the characteristic equation),
        then the solution to the recurrence relation is
        <me permid="Mis">
          a_n = ar_1^n + br_2^n
        </me>,
        where <m>a</m> and <m>b</m> are constants determined by the initial conditions.
      </p>
        </assemblage>
      </slide>
      <slide>
        <example source-number="2.4.6">
          <statement>
            <p permid="uAn">
          Solve the recurrence relation
          <m>a_n = 7a_{n-1} - 10 a_{n-2}</m> with <m>a_0 = 2</m> and <m>a_1 = 3</m>.
        </p>
          </statement>
        </example>
      </slide>
      <slide>
        <assemblage>
          <title>Characteristic Root Technique for Repeated Roots</title>
          <p permid="oLb">
        Suppose the recurrence relation
        <m>a_n = \alpha a_{n-1} + \beta a_{n-2}</m> has a characteristic polynomial with only one root <m>r</m>.
        Then the solution to the recurrence relation is
        <me permid="QSl">
          a_n = ar^n + bnr^n
        </me>
        where <m>a</m> and <m>b</m> are constants determined by the initial conditions.
      </p>
        </assemblage>
      </slide>
      <slide>
        <example source-number="2.4.7">
          <statement>
            <p permid="aHw">
          Solve the recurrence relation
          <m>a_n = 6a_{n-1} - 9a_{n-2}</m> with initial conditions <m>a_0 = 1</m> and <m>a_1 = 4</m>.
        </p>
          </statement>
        </example>
      </slide>
    </subsection>
  </slideshow>
</pretext>
